

# Algebra from a Categorical Perspective

Saxon Supple

February 2026

## 1 Introduction

This article will give categorical definitions of the standard objects from algebra, by way of defining universal properties which determine the objects up to unique isomorphism. For a given object  $A$  of interest, the general procedure will be to first define an object  $B$  as an object which satisfies a specific universal property, then show that  $A$  satisfies that universal property, and then show that all pairs of objects  $B$  which satisfy the universal property are related by a unique isomorphism. This will then demonstrate that the universal property determines  $A$  up to unique isomorphism. We will then apply these universal properties to prove additional useful categorical results, such as the functoriality of the abelianization of a group.

## 2 Preliminary Categorical Constructions

**Definition 2.1.** Let  $\mathbf{C}$  be a category and let  $f_1, f_2 : X \rightarrow Y \in \text{Hom}_{\mathbf{C}}(X, Y)$ . Then a morphism  $j : W \rightarrow X \in \text{Hom}_{\mathbf{C}}(W, X)$  is an equaliser of  $f_1$  and  $f_2$  if  $f_1 \circ j = f_2 \circ j$  and given any morphism  $g : T \rightarrow X$  with  $f_1 \circ g = f_2 \circ g$ , there is a unique morphism  $h : T \rightarrow W$  such that  $j \circ h = g$ .

$$\begin{array}{ccccc} W & \xrightarrow{j} & X & \xrightarrow[f_2]{f_1} & Y \\ \uparrow \exists! h & \nearrow \forall g & & & \\ T & & & & \end{array}$$

**Theorem 2.2.** Let  $\mathbf{C}$  be a category, and suppose that  $j : W \rightarrow X$  and  $j' : W' \rightarrow X$  are both equalizers of morphisms  $f_1, f_2 \in \text{Hom}_{\mathbf{C}}(X, Y)$ . Then there exists a unique isomorphism  $h : W \rightarrow W'$  such that  $j = j' \circ h$ .

*Proof.* Since  $j'$  is an equalizer and  $f_1 \circ j = f_2 \circ j$ , there exists a unique morphism  $h : W \rightarrow W'$  such that  $j = j' \circ h$ . Similarly, there exists a unique morphism  $h' : W' \rightarrow W$  such that  $j' = j \circ h'$ . Hence, we have  $j' = j' \circ (h \circ h')$ . If we then let  $T = W'$  and  $g = j'$ , since we have that both  $j' \circ \text{id}_{W'} = j'$  and  $j' \circ (h \circ h') = j'$ , it follows from uniqueness that  $h \circ h' = \text{id}_{W'}$ . Similarly,  $h' \circ h = \text{id}_W$ . Hence,  $h$  is an isomorphism.  $\square$

**Definition 2.3.** Let  $\mathbf{C}$  be a category and let  $f_1, f_2 : X \rightarrow Y$  be morphisms. Then a morphism  $q : Y \rightarrow Z$  is a coequalizer of  $f_1$  and  $f_2$  if  $q \circ f_1 = q \circ f_2$  and if  $g : Y \rightarrow W$  is a morphism with

$g \circ f_1 = g \circ f_2$ , then there is a unique morphism  $h : Z \rightarrow W$  with  $g = h \circ q$ .

$$\begin{array}{ccccc} X & \xrightarrow{f_1} & Y & \xrightarrow{q} & Z \\ & \searrow f_2 & & \searrow & \downarrow \exists! h \\ & & & & W \end{array}$$

**Theorem 2.4.** Let  $\mathbf{C}$  be a category, and let  $q : Y \rightarrow Z$  and  $q' : Y \rightarrow Z'$  both be coequalizers of  $f_1, f_2 \in \text{Hom}_{\mathbf{C}}(X, Y)$ . Then there is a unique isomorphism  $h : Z \rightarrow Z'$  such that  $q' = h \circ q$ .

*Proof.* Since  $q$  is a coequalizer and  $q' \circ f_1 = q' \circ f_2$ , there exists a unique morphism  $h : Z \rightarrow Z'$  such that  $q' = h \circ q$ . Similarly, there exists a unique morphism  $h' : Z' \rightarrow Z$  such that  $q = h' \circ q'$ . Hence, we have  $q' = (h \circ h') \circ q'$ . If we then let  $W = Z'$  and  $g = q'$ , since we have that both  $\text{id}_{Z'} \circ q' = q'$  and  $q' = (h \circ h') \circ q'$ , it follows from uniqueness that  $h \circ h' = \text{id}_{Z'}$ . Similarly,  $h' \circ h = \text{id}_Z$ . Hence,  $h$  is an isomorphism.  $\square$

**Definition 2.5.** Let  $\mathbf{C}$  be a category, and let  $(X_\alpha)_{\alpha \in \mathcal{A}}$  be an indexed collection of objects of  $\mathbf{C}$ . An object  $X$  equipped with morphisms  $\text{pr}_\alpha : X \rightarrow X_\alpha$  is a product of  $(X_\alpha)_{\alpha \in \mathcal{A}}$  if for any object  $Z$  and morphisms  $f_\alpha : Z \rightarrow X_\alpha$ , there exists a unique morphism  $F : Z \rightarrow X$  such that  $\text{pr}_\alpha \circ F = f_\alpha \forall \alpha \in \mathcal{A}$ .

$$\begin{array}{ccc} & Z & \\ f_1 \swarrow & \downarrow \exists! F & \searrow f_2 \\ & X & \\ \text{pr}_1 \swarrow & & \searrow \text{pr}_2 \\ X_1 & & X_2 \end{array}$$

**Theorem 2.6.** Let  $\mathbf{C}$  be a category, and let  $(X_\alpha)_{\alpha \in \mathcal{A}}$  be an indexed collection of objects of  $\mathbf{C}$ . Suppose  $(X, \text{pr}_\alpha)$  and  $(X', \text{pr}'_\alpha)$  are both products of  $(X_\alpha)_{\alpha \in \mathcal{A}}$ . Then there exists a unique isomorphism  $h : X \rightarrow X'$  such that  $\text{pr}'_\alpha \circ h = \text{pr}_\alpha \forall \alpha \in \mathcal{A}$ .

*Proof.* If we let  $Z = X'$  and  $f_\alpha = \text{pr}'_\alpha$ , then there exists a unique morphism  $h' : X' \rightarrow X$  such that  $\text{pr}'_\alpha = \text{pr}_\alpha \circ h'$ . Similarly, there exists a unique morphism  $h : X \rightarrow X'$  such that  $\text{pr}_\alpha = \text{pr}'_\alpha \circ h$ . From this we obtain  $\text{pr}_\alpha = \text{pr}_\alpha \circ (h' \circ h)$ . Then, if we let  $Z = X$  and  $f_\alpha = \text{pr}_\alpha$ , we see that both  $h' \circ h$  and  $\text{id}_X$  are candidates for  $F$ . Hence, by uniqueness,  $h' \circ h = \text{id}_X$ . Similarly,  $h \circ h' = \text{id}_{X'}$ . Hence,  $h$  is an isomorphism.  $\square$

**Definition 2.7.** Let  $\mathbf{C}$  be a category and let  $(X_\alpha)_{\alpha \in \mathcal{A}}$  be an indexed collection of objects of  $\mathbf{C}$ . An object  $Y$  along with morphisms  $\iota_\alpha : X_\alpha \rightarrow Y$  is a coproduct of  $(X_\alpha)_{\alpha \in \mathcal{A}}$  if for any object  $Z$  with morphisms  $f_\alpha : X_\alpha \rightarrow Z$ , there exists a unique morphism  $F : Y \rightarrow Z$  such that for all  $\alpha \in \mathcal{A}$ , we have  $F \circ \iota_\alpha = f_\alpha$ .

$$\begin{array}{ccc} X_1 & & X_2 \\ & \searrow \iota_1 & \swarrow \iota_2 \\ & Y & \\ f_1 \swarrow & \downarrow \exists! F & \searrow f_2 \\ & Z & \end{array}$$

**Theorem 2.8.** *Let  $\mathbf{C}$  be a category and let  $(X_\alpha)_{\alpha \in \mathcal{A}}$  be objects of  $\mathbf{C}$ . Suppose that both  $(Y, (\iota_\alpha)_{\alpha \in \mathcal{A}})$  and  $(Y', (\iota'_\alpha)_{\alpha \in \mathcal{A}})$  are coproducts of  $(X_\alpha)_{\alpha \in \mathcal{A}}$ . Then there exists a unique isomorphism  $h : Y \rightarrow Y'$  such that  $h \circ \iota_\alpha = \iota'_\alpha \forall \alpha \in \mathcal{A}$ .*

*Proof.* If we let  $Z = Y'$  and  $f_\alpha = \iota'_\alpha$ , there exists a unique morphism  $h : Y \rightarrow Y'$  such that  $\iota'_\alpha = h \circ \iota_\alpha \forall \alpha \in \mathcal{A}$ . Similarly, there exists a unique morphism  $h' : Y' \rightarrow Y$  such that  $\iota_\alpha = h' \circ \iota'_\alpha \forall \alpha \in \mathcal{A}$ . Hence, we have  $\iota_\alpha = (h' \circ h) \circ \iota_\alpha \forall \alpha \in \mathcal{A}$ . If we then let  $Z = Y$  and  $f_\alpha = \iota_\alpha$ , we see that both  $h' \circ h$  and  $\text{id}_Y$  are candidates for  $F$ . Hence, by uniqueness,  $h' \circ h = \text{id}_Y$ . Similarly,  $h \circ h' = \text{id}_{Y'}$ . Hence,  $h$  is an isomorphism.  $\square$

### 3 Sets

**Definition 3.1.** *Let  $X$  be a set, and let  $\sim$  be an equivalence relation on  $X$ . We say that a function  $f : X \rightarrow Y$  is  $\sim$ -invariant if  $x_0 \sim x_1 \implies f(x_0) = f(x_1) \forall x_0, x_1 \in X$ .*

**Definition 3.2** (Universal property of the quotient set). *Let  $X$  be a set and let  $\sim$  be an equivalence relation on  $X$ . A pair  $(X', \pi : X \rightarrow X')$  is a quotient of  $X$  by  $\sim$  if  $\pi$  is  $\sim$ -invariant, and given any  $\sim$ -invariant function  $f : X \rightarrow Y$ , there exists a unique  $\bar{f} : X' \rightarrow Y$  such that  $f = \bar{f} \circ \pi$ .*

**Theorem 3.3.** *The canonical projection  $\pi : X \rightarrow X/\sim : x \mapsto [x]$  satisfies the universal property of the quotient set.*

*Proof.* First note that  $\pi$  is clearly  $\sim$ -invariant. We define  $\bar{f} : X/\sim \rightarrow Y$  by  $\bar{f}(\pi(x)) = f(x)$ . This is well-defined, since if  $x_0 \sim x_1$ , then  $\bar{f}(\pi(x_0)) = f(x_0) = f(x_1) = \bar{f}(\pi(x_1))$ , and hence  $\bar{f}$  is independent of representatives. Uniqueness is also evident from the definition of  $\pi$ .  $\square$

**Theorem 3.4.** *Let  $X$  be a set with an equivalence relation  $\sim$ . Let  $(W, \pi_W)$  and  $(Z, \pi_Z)$  be two pairs of sets, along with maps  $\pi_W : X \rightarrow W$  and  $\pi_Z : X \rightarrow Z$  such that both pairs satisfy the universal property of the quotient set. Then there exists a unique bijection  $h : W \rightarrow Z$  such that  $\pi_Z = h \circ \pi_W$ .*

*Proof.* Let  $(X', \pi : X \rightarrow X')$  be a quotient of  $X$  by  $\sim$ . Let  $R \subseteq X \times X$  be defined as  $R = \{(x_0, x_1) : x_0 \sim x_1\}$ . Then define  $\text{pr}_1 : R \rightarrow X : (x_0, x_1) \mapsto x_0$  and  $\text{pr}_2 : R \rightarrow X : (x_0, x_1) \mapsto x_1$ . We then note that  $\sim$ -invariance of a function  $g : X \rightarrow Y$  is equivalent to the property that  $g \circ \text{pr}_1 = g \circ \text{pr}_2$ . We then have that  $\pi \circ \text{pr}_1 = \pi \circ \text{pr}_2$ , and given any  $f : X \rightarrow Y$  such that  $f \circ \text{pr}_1 = f \circ \text{pr}_2$ , there exists a unique  $\bar{f} : X' \rightarrow Y$  such that  $f = \bar{f} \circ \pi$ .

$$\begin{array}{ccccc} R & \xrightarrow[\text{pr}_2]{\text{pr}_1} & X & \xrightarrow{\pi} & X' \\ & & & \searrow & \downarrow \exists! \bar{f} \\ & & & \forall f & Y \end{array}$$

This is identical to saying that  $\pi$  is a coequalizer of  $\text{pr}_1$  and  $\text{pr}_2$  in the category of sets, and hence,  $\pi$  is unique up to unique bijection. In particular, there exists a unique bijection  $h : W \rightarrow Z$  such that  $\pi_Z = h \circ \pi_W$ .  $\square$

## 4 Groups

### 4.1 Quotient Groups

**Definition 4.1** (Universal property of the quotient group). *Let  $G$  be a group, and let  $N \trianglelefteq G$  be a normal subgroup. A pair  $(Q, q : G \rightarrow Q)$ , consisting of a group  $Q$  and a group homomorphism  $q$ , is*

a quotient of  $G$  if  $N \subseteq \ker q$  and given any group homomorphism  $\phi : G \rightarrow H$  with  $N \subseteq \ker \phi$ , there exists a unique group homomorphism  $\bar{\phi} : Q \rightarrow H$  such that  $\phi = \bar{\phi} \circ q$ .

**Theorem 4.2.** Let  $G$  be a group and let  $N \trianglelefteq G$  be a normal subgroup. Then the canonical quotient homomorphism  $\pi : G \rightarrow G/N : g \mapsto gN$  is a quotient homomorphism.

*Proof.* Let  $\sim$  be an equivalence relation on  $G$  which identifies the fibres of  $\pi$ ; that is,  $x \sim y \iff xN = yN$ . If  $\pi(x) = \pi(y)$ , then  $x$  and  $y$  are in the same coset, so there exists some  $n \in N$  such that  $x = yn$ . Hence, since  $N \subseteq \ker \phi$ , we have  $\phi(x) = \phi(yn) = \phi(y)\phi(n) = \phi(y)$ . Then by the universal property of the quotient set, there exists a unique map  $\bar{\phi} : G/\sim \rightarrow H$  such that  $\phi = \bar{\phi} \circ \pi$ . In particular,  $\bar{\phi}$  is defined as  $\bar{\phi}([x]) = \bar{\phi}(xN) = \phi(x)\forall x$ , and hence  $\bar{\phi}$  is simply a map on the cosets of  $N$ . Furthermore, given  $x, y \in G$ , we have  $\bar{\phi}(xyN) = \phi(xy) = \phi(x)\phi(y) = \bar{\phi}(xN)\bar{\phi}(yN)$ , and hence  $\bar{\phi}$  is a group homomorphism.  $\square$

**Corollary 4.3.** Let  $\phi : G \rightarrow H$  be a group homomorphism, and let  $N \trianglelefteq G$  be a normal subgroup such that  $N \subseteq \ker \phi$ . Then  $N = \ker \phi$  if and only if  $\bar{\phi} : G/N \rightarrow H$  is injective.

*Proof.* By the universal property of the quotient group, we know that  $\bar{\phi}$  is both unique and well-defined. First suppose that  $N = \ker \phi$ . Let  $gN \in \ker \bar{\phi}$ . Then  $\phi(g) = \bar{\phi}(gN) = e$ , and hence  $g \in \ker \phi = N$ , implying that  $gN = N$ . Hence,  $\ker \bar{\phi} = N$ , implying that  $\bar{\phi}$  is injective. Now suppose that  $\bar{\phi}$  is injective. That then means that  $\ker \bar{\phi} = N$ . Let  $g \in \ker \phi$ . Then  $\bar{\phi}(gN) = \phi(g) = e$ , implying that  $gN = N$ , or  $g \in N$ . Hence,  $N = \ker \phi$ .  $\square$

**Theorem 4.4.** Let  $G$  be a group and let  $N \trianglelefteq G$  be a normal subgroup. Let  $q : G \rightarrow Q$  and  $q' : G \rightarrow Q'$  be two quotient homomorphisms. Then there exists a unique isomorphism  $h : Q \rightarrow Q'$  such that  $q' = h \circ q$ .

*Proof.* Let  $\pi : G \rightarrow K$  be a quotient homomorphism. Let  $\iota : N \hookrightarrow G$  be the inclusion homomorphism, and let  $z : N \rightarrow G : n \mapsto e$  be the trivial homomorphism. Then  $\pi \circ \iota = \pi \circ z \iff \pi(n) = e\forall n \in N \iff N \subseteq \ker \pi$ , which is true by the definition of  $\pi$ . Let  $\phi : G \rightarrow H$  be any homomorphism with  $N \subseteq \ker \phi$ , or in other words, with  $\phi \circ \iota = \phi \circ z$ . Then by the universal property, there exists a unique homomorphism  $\bar{\phi} : K \rightarrow H$  such that  $\phi = \bar{\phi} \circ \pi$ .

$$\begin{array}{ccccc} N & \xrightarrow{\iota} & G & \xrightarrow{\pi} & K \\ & & \searrow & & \downarrow \exists! \bar{\phi} \\ & & & & H \end{array}$$

$\forall \phi$

This is exactly equivalent to saying that  $\pi$  is a coequalizer in the category of groups. Hence, the result follows by uniqueness.  $\square$

## 4.2 Products

## 4.3 Abelianization

**Definition 4.5** (Universal property of the abelianization of a group). Let  $G$  be a group. An abelianization of  $G$  is a pair  $(G^{ab}, \pi)$ , where  $G^{ab}$  is an abelian group and  $\pi : G \rightarrow G^{ab}$  is a group homomorphism, such that given any abelian group  $H$  and group homomorphism  $\phi : G \rightarrow H$ , there exists a unique group homomorphism  $\phi^{ab} : G^{ab} \rightarrow H$  such that  $\phi^{ab} \circ \pi = \phi$ .

**Theorem 4.6.** Let  $G$  be a group, let  $[G, G]$  be the commutator subgroup, and let  $\pi : G \rightarrow G/[G, G]$  be the canonical quotient homomorphism. Then  $(G/[G, G], \pi)$  is an abelianization of  $G$ .

*Proof.* We simply need to show that the commutator subgroup  $[G, G]$  is contained within the kernel of  $\phi$ , since that will allow us to apply the universal property of the quotient group to obtain the unique group homomorphism  $\phi^{\text{ab}} : G/[G, G] \rightarrow H$  such that  $\phi^{\text{ab}} \circ \pi = \phi$ . Indeed, let  $x, y \in G$ . Then  $\phi([x, y]) = \phi(x^{-1}y^{-1}xy) = \phi(x)^{-1}\phi(y)^{-1}\phi(x)\phi(y) = e$ , so  $[x, y] \in \ker \phi$ . Hence, since  $[G, G]$  is the subgroup generated by all commutators, it follows that  $[G, G] \subseteq \ker \phi$ , as required.  $\square$

**Theorem 4.7.** *Let  $G$  be a group, and let  $(G^{\text{ab}}, \pi)$  and  $(G^{\text{ab}'}, \pi')$  be two abelianizations of  $G$ . Then there exists a unique isomorphism  $h : G^{\text{ab}} \rightarrow G^{\text{ab}'}$  such that  $\pi' = h \circ \pi$ .*

*Proof.* By the universal property of the abelianization of a group, there exists a unique group isomorphism  $h : G^{\text{ab}} \rightarrow G^{\text{ab}'}$  such that  $\pi' = h \circ \pi$ . Similarly, there exists a unique group isomorphism  $g : G^{\text{ab}'} \rightarrow G^{\text{ab}}$  such that  $\pi = g \circ \pi'$ . Hence,  $\pi' = (h \circ g) \circ \pi'$ . However, we also have  $\pi' = \text{id}_{G^{\text{ab}'}} \circ \pi'$ , and hence, by uniqueness, we have  $h \circ g = \text{id}_{G^{\text{ab}'}}$ . Similarly,  $g \circ h = \text{id}_{G^{\text{ab}}}$ , implying that  $h$  is an isomorphism.  $\square$

**Lemma 4.8.** *Let  $\phi : G \rightarrow H$  be a group homomorphism, and let  $\pi_G : G \rightarrow G/[G, G]$ ,  $\pi_H : H \rightarrow H/[H, H]$  be the quotient homomorphisms of  $G$  and  $H$  into their respective abelianizations. Then there exists a group homomorphism  $\phi^{\text{ab}} : G^{\text{ab}} \rightarrow H^{\text{ab}}$  given by  $\phi^{\text{ab}}(g[G, G]) = \phi(g)[H, H] \forall g[G, G] \in G^{\text{ab}}$ , which is the unique group homomorphism  $\psi : G^{\text{ab}} \rightarrow H^{\text{ab}}$  such that  $\psi \circ \pi_G = \pi_H \circ \phi$ .*

*Proof.* Consider the map  $\pi_H \circ \phi : G \rightarrow H^{\text{ab}}$ . This is a map from a group to an abelian group, so by the universal property of the abelianization of a group, there exists a unique group homomorphism  $\phi^{\text{ab}} : G^{\text{ab}} \rightarrow H^{\text{ab}}$  such that  $\phi^{\text{ab}} \circ \pi_G = \pi_H \circ \phi$ . That is, given any  $g \in G$ , we have

$$\phi^{\text{ab}}(g[G, G]) = \phi^{\text{ab}} \circ \pi_G(g) = \pi_H \circ \phi(g) = \phi(g)[H, H],$$

as required.  $\square$

**Theorem 4.9.** *There is a covariant functor, called the abelianization functor, from the category of groups to the category of abelian groups.*

*Proof.* Let  $F$  be the functor which maps groups to their abelianizations, and group homomorphisms to group homomorphisms between the abelianizations of the groups. That is, given groups  $G$  and  $H$  and a group homomorphism  $\phi : G \rightarrow H$ , we have  $F(G) = G^{\text{ab}}$  and  $F(\phi) = \phi^{\text{ab}} : G^{\text{ab}} \rightarrow H^{\text{ab}} : g[G, G] \mapsto \phi(g)[H, H]$ .

We first show that  $F(\text{id}_G) = \text{id}_{F(G)}$  for any group  $G$ . Indeed,  $F(\text{id}_G)$  is given by  $\text{id}_{G^{\text{ab}}} : G^{\text{ab}} \rightarrow G^{\text{ab}}$ , where  $\text{id}_{G^{\text{ab}}}(g[G, G]) = \text{id}_G(g)[G, G] = g[G, G] \forall g \in G$ .  $F(\text{id}_G)$  is then the identity map on  $G^{\text{ab}} = F(G)$ , as required.

We now show that  $F$  preserves composition. Let  $G, H, K$  be groups and let  $\phi : G \rightarrow H$  and  $\psi : H \rightarrow K$  be group homomorphisms. Then

$$F(\phi) = \phi^{\text{ab}} : G^{\text{ab}} \rightarrow H^{\text{ab}} : g[G, G] \mapsto \phi(g)[H, H],$$

$$F(\psi) = \psi^{\text{ab}} : H^{\text{ab}} \rightarrow K^{\text{ab}} : h[H, H] \mapsto \psi(h)[K, K]$$

and

$$F(\psi \circ \phi) = (\psi \circ \phi)^{\text{ab}} : G^{\text{ab}} \rightarrow K^{\text{ab}} : g[G, G] \mapsto (\psi \circ \phi)(g)[K, K].$$

Hence,

$$\begin{aligned}(\psi^{\text{ab}} \circ \phi^{\text{ab}})(g[G, G]) &= \psi^{\text{ab}}(\phi(g)[H, H]) \\&= \psi(\phi(g))[K, K] \\&= (\psi \circ \phi)(g)[K, K] \\&= (\psi \circ \phi)^{\text{ab}}(g[G, G]),\end{aligned}$$

as required. Hence,  $F$  is a covariant functor. □